F_mu_ref/fundamental_binary.v
@@ -1,0 +1,314 @@
+From iris_logrel.F_mu_ref Require Export logrel_binary.
+From iris.proofmode Require Import tactics.
+From iris_logrel.F_mu_ref Require Import rules_binary.
+From iris.base_logic Require Export big_op.
+
+Section bin_log_def.
+  Context `{cfgSG Σ}.
+  Notation D := (prodC valC valC -n> iProp Σ).
+
+  Definition bin_log_related (Γ : list type) (e e' : expr) (τ : type) := ∀ Δ vvs ρ,
+    env_PersistentP Δ →
+    heap_ctx ∧ spec_ctx ρ ∧
+    ⟦ Γ ⟧* Δ vvs ⊢ ⟦ τ ⟧ₑ Δ (e.[env_subst (vvs.*1)], e'.[env_subst (vvs.*2)]).
+End bin_log_def.
+
+Notation "Γ ⊨ e '≤log≤' e' : τ" :=
+  (bin_log_related Γ e e' τ) (at level 74, e, e', τ at next level).
+
+Section fundamental.
+  Context `{cfgSG Σ}.
+  Notation D := (prodC valC valC -n> iProp Σ).
+  Implicit Types e : expr.
+  Implicit Types Δ : listC D.
+  Hint Resolve to_of_val.
+
+  Local Tactic Notation "smart_wp_bind" uconstr(ctx) ident(v) ident(w)
+        constr(Hv) uconstr(Hp) :=
+    iApply (wp_bind [ctx]);
+    iApply wp_wand_l; iSplitR;
+    [|iApply Hp; rewrite ?fill_app /=; iFrame "#"; trivial];
+    let Htmp := iFresh in
+    iIntros (v) Htmp; iDestruct Htmp as (w) Hv;
+    rewrite fill_app; simpl.
+
+  Local Ltac value_case := iApply wp_value; [cbn; rewrite ?to_of_val; trivial|].
+
+  (* Put all quantifiers at the outer level *)
+  Lemma bin_log_related_alt {Γ e e' τ} : Γ ⊨ e ≤log≤ e' : τ → ∀ Δ vvs ρ K,
+    env_PersistentP Δ →
+    heap_ctx ∗ spec_ctx ρ ∗ ⟦ Γ ⟧* Δ vvs ∗ ⤇ fill K (e'.[env_subst (vvs.*2)])
+    ⊢ WP e.[env_subst (vvs.*1)] {{ v, ∃ v',
+        ⤇ fill K (of_val v') ∗ interp τ Δ (v, v') }}.
+  Proof.
+    iIntros (Hlog Δ vvs ρ K ?) "(#Hh & #Hs & HΓ & Hj)".
+    iApply (Hlog with "[HΓ] *"); iFrame; eauto.
+  Qed.
+
+  Notation "' H" := (bin_log_related_alt H) (at level 8).
+
+  Lemma bin_log_related_var Γ x τ :
+    Γ !! x = Some τ → Γ ⊨ Var x ≤log≤ Var x : τ.
+  Proof.
+    iIntros (? Δ vvs ρ ?) "#(Hh & Hs & HΓ)"; iIntros (K) "Hj /=".
+    iDestruct (interp_env_Some_l with "HΓ") as ([v v']) "[% ?]"; first done.
+    rewrite /env_subst !list_lookup_fmap; simplify_option_eq. value_case; eauto.
+  Qed.
+
+  Lemma bin_log_related_unit Γ : Γ ⊨ Unit ≤log≤ Unit : TUnit.
+  Proof.
+    iIntros (Δ vvs ρ ?) "#(Hh & Hs & HΓ)"; iIntros (K) "Hj /=".
+    value_case. iExists UnitV; eauto.
+  Qed.
+
+  Lemma bin_log_related_pair Γ e1 e2 e1' e2' τ1 τ2
+      (IHHtyped1 : Γ ⊨ e1 ≤log≤ e1' : τ1)
+      (IHHtyped2 : Γ ⊨ e2 ≤log≤ e2' : τ2) :
+    Γ ⊨ Pair e1 e2 ≤log≤ Pair e1' e2' : TProd τ1 τ2.
+  Proof.
+    iIntros (Δ vvs ρ ?) "#(Hh & Hs & HΓ)"; iIntros (K) "Hj /=".
+    smart_wp_bind (PairLCtx e2.[env_subst _]) v v' "[Hv #Hiv]"
+      ('IHHtyped1 _ _ _ (K ++ [PairLCtx e2'.[env_subst _] ])).
+    smart_wp_bind (PairRCtx v) w w' "[Hw #Hiw]"
+      ('IHHtyped2 _ _ _ (K ++ [PairRCtx v'])).
+    value_case. iExists (PairV v' w'); iFrame "Hw".
+    iExists (v, v'), (w, w'); simpl; repeat iSplit; trivial.
+  Qed.
+
+  Lemma bin_log_related_fst Γ e e' τ1 τ2
+      (IHHtyped : Γ ⊨ e ≤log≤ e' : TProd τ1 τ2) :
+    Γ ⊨ Fst e ≤log≤ Fst e' : τ1.
+  Proof.
+    iIntros (Δ vvs ρ ?) "#(Hh & Hs & HΓ)"; iIntros (K) "Hj /=".
+    smart_wp_bind (FstCtx) v v' "[Hv #Hiv]" ('IHHtyped _ _ _ (K ++ [FstCtx])); cbn.
+    iDestruct "Hiv" as ([w1 w1'] [w2 w2']) "#[% [Hw1 Hw2]]"; simplify_eq.
+    iMod (step_fst _ _ K (of_val w1') w1' (of_val w2') w2' with "* [-]") as "Hw"; eauto.
+    iApply wp_fst; eauto.
+  Qed.
+
+  Lemma bin_log_related_snd Γ e e' τ1 τ2
+      (IHHtyped : Γ ⊨ e ≤log≤ e' : TProd τ1 τ2) :
+    Γ ⊨ Snd e ≤log≤ Snd e' : τ2.
+  Proof.
+    iIntros (Δ vvs ρ ?) "#(Hh & Hs & HΓ)"; iIntros (K) "Hj /=".
+    smart_wp_bind (SndCtx) v v' "[Hv #Hiv]" ('IHHtyped _ _ _ (K ++ [SndCtx])); cbn.
+    iDestruct "Hiv" as ([w1 w1'] [w2 w2']) "#[% [Hw1 Hw2]]"; simplify_eq.
+    iMod (step_snd _ _ K (of_val w1') w1' (of_val w2') w2' with "* [-]") as "Hw"; eauto.
+    iApply wp_snd; eauto.
+  Qed.
+
+  Lemma bin_log_related_injl Γ e e' τ1 τ2
+      (IHHtyped : Γ ⊨ e ≤log≤ e' : τ1) :
+    Γ ⊨ InjL e ≤log≤ InjL e' : (TSum τ1 τ2).
+  Proof.
+    iIntros (Δ vvs ρ ?) "#(Hh & Hs & HΓ)"; iIntros (K) "Hj /=".
+    smart_wp_bind (InjLCtx) v v' "[Hv #Hiv]"
+      ('IHHtyped _ _ _ (K ++ [InjLCtx])); cbn.
+    value_case. iExists (InjLV v'); iFrame "Hv".
+    iLeft; iExists (_,_); eauto 10.
+  Qed.
+
+  Lemma bin_log_related_injr Γ e e' τ1 τ2
+      (IHHtyped : Γ ⊨ e ≤log≤ e' : τ2) :
+    Γ ⊨ InjR e ≤log≤ InjR e' : TSum τ1 τ2.
+  Proof.
+    iIntros (Δ vvs ρ ?) "#(Hh & Hs & HΓ)"; iIntros (K) "Hj /=".
+    smart_wp_bind (InjRCtx) v v' "[Hv #Hiv]"
+      ('IHHtyped _ _ _ (K ++ [InjRCtx])); cbn.
+    value_case. iExists (InjRV v'); iFrame "Hv".
+    iRight; iExists (_,_); eauto 10.
+  Qed.
+
+  Lemma bin_log_related_case Γ e0 e1 e2 e0' e1' e2' τ1 τ2 τ3
+      (Hclosed2 : ∀ f, e1.[upn (S (length Γ)) f] = e1)
+      (Hclosed3 : ∀ f, e2.[upn (S (length Γ)) f] = e2)
+      (Hclosed2' : ∀ f, e1'.[upn (S (length Γ)) f] = e1')
+      (Hclosed3' : ∀ f, e2'.[upn (S (length Γ)) f] = e2')
+      (IHHtyped1 : Γ ⊨ e0 ≤log≤ e0' : TSum τ1 τ2)
+      (IHHtyped2 : τ1 :: Γ ⊨ e1 ≤log≤ e1' : τ3)
+      (IHHtyped3 : τ2 :: Γ ⊨ e2 ≤log≤ e2' : τ3) :
+    Γ ⊨ Case e0 e1 e2 ≤log≤ Case e0' e1' e2' : τ3.
+  Proof.
+    iIntros (Δ vvs ρ ?) "#(Hh & Hs & HΓ)"; iIntros (K) "Hj /=".
+    iDestruct (interp_env_length with "HΓ") as %?.
+    smart_wp_bind (CaseCtx _ _) v v' "[Hv #Hiv]"
+      ('IHHtyped1 _ _ _ (K ++ [CaseCtx _ _])); cbn.
+    iDestruct "Hiv" as "[Hiv|Hiv]".
+    - iDestruct "Hiv" as ([w w']) "[% Hw]"; simplify_eq.
+      iMod (step_case_inl _ _ K (of_val w') w' with "* [-]") as "Hz"; eauto.
+      iApply wp_case_inl; auto 1 using to_of_val. iNext.
+      asimpl. erewrite !n_closed_subst_head_simpl by (rewrite ?fmap_length; eauto).
+      iApply ('IHHtyped2 _ ((w,w') :: vvs)); repeat iSplit; eauto.
+      iApply interp_env_cons; auto.
+    - iDestruct "Hiv" as ([w w']) "[% Hw]"; simplify_eq.
+      iMod (step_case_inr _ _ K (of_val w') w' with "* [-]") as "Hz"; eauto.
+      iApply wp_case_inr; auto 1 using to_of_val. iNext.
+      asimpl. erewrite !n_closed_subst_head_simpl by (rewrite ?fmap_length; eauto).
+      iApply ('IHHtyped3 _ ((w,w') :: vvs)); repeat iSplit; eauto.
+      iApply interp_env_cons; auto.
+  Qed.
+
+  Lemma bin_log_related_lam Γ (e e' : expr) τ1 τ2
+      (Hclosed : ∀ f, e.[upn (S (length Γ)) f] = e)
+      (Hclosed' : ∀ f, e'.[upn (S (length Γ)) f] = e')
+      (IHHtyped : τ1 :: Γ ⊨ e ≤log≤ e' : τ2) :
+    Γ ⊨ Lam e ≤log≤ Lam e' : TArrow τ1 τ2.
+  Proof.
+    iIntros (Δ vvs ρ ?) "#(Hh & Hs & HΓ)"; iIntros (K) "Hj /=".
+    value_case. iExists (LamV _). iIntros "{$Hj} !#".
+    iIntros ([v v']) "#Hiv". iIntros (K') "Hj".
+    iDestruct (interp_env_length with "HΓ") as %?.
+    iApply wp_lam; auto 1 using to_of_val. iNext.
+    iMod (step_lam _ _ K' _ (of_val v') v' with "* [-]") as "Hz"; eauto.
+    asimpl. erewrite !n_closed_subst_head_simpl by (rewrite ?fmap_length; eauto).
+    iApply ('IHHtyped _ ((v,v') :: vvs)); repeat iSplit; eauto.
+    iApply interp_env_cons; iSplit; auto.
+  Qed.
+
+  Lemma bin_log_related_app Γ e1 e2 e1' e2' τ1 τ2
+      (IHHtyped1 : Γ ⊨ e1 ≤log≤ e1' : TArrow τ1 τ2)
+      (IHHtyped2 : Γ ⊨ e2 ≤log≤ e2' : τ1) :
+    Γ ⊨ App e1 e2 ≤log≤ App e1' e2' :  τ2.
+  Proof.
+    iIntros (Δ vvs ρ ?) "#(Hh & Hs & HΓ)"; iIntros (K) "Hj /=".
+    smart_wp_bind (AppLCtx (e2.[env_subst (vvs.*1)])) v v' "[Hv #Hiv]"
+      ('IHHtyped1 _ _ _ (K ++ [(AppLCtx (e2'.[env_subst (vvs.*2)]))])); cbn.
+    smart_wp_bind (AppRCtx v) w w' "[Hw #Hiw]"
+                  ('IHHtyped2 _ _ _ (K ++ [AppRCtx v'])); cbn.
+    iApply ("Hiv" $! (w, w') with "Hiw *"); simpl; eauto.
+  Qed.
+
+  Lemma bin_log_related_tlam Γ e e' τ
+      (IHHtyped : (subst (ren (+1)) <$> Γ) ⊨ e ≤log≤ e' : τ) :
+    Γ ⊨ TLam e ≤log≤ TLam e' : TForall τ.
+  Proof.
+    iIntros (Δ vvs ρ ?) "#(Hh & Hs & HΓ)"; iIntros (K) "Hj /=".
+    value_case. iExists (TLamV _).
+    iIntros "{$Hj} /= !#"; iIntros (τi ? K') "Hv /=".
+    iApply wp_tlam; iNext.
+    iMod (step_tlam _ _ K' (e'.[env_subst (vvs.*2)]) with "* [-]") as "Hz"; eauto.
+    iApply 'IHHtyped; repeat iSplit; eauto. by iApply interp_env_ren.
+  Qed.
+
+  Lemma bin_log_related_tapp Γ e e' τ τ'
+      (IHHtyped : Γ ⊨ e ≤log≤ e' : TForall τ) :
+    Γ ⊨ TApp e ≤log≤ TApp e' : τ.[τ'/].
+  Proof.
+    iIntros (Δ vvs ρ ?) "#(Hh & Hs & HΓ)"; iIntros (K) "Hj /=".
+    smart_wp_bind (TAppCtx) v v' "[Hj #Hv]"
+      ('IHHtyped _ _ _ (K ++ [TAppCtx])); cbn.
+    iApply wp_wand_r; iSplitL.
+    { iSpecialize ("Hv" $! (interp τ' Δ) with "[#]"); [iPureIntro; apply _|].
+      iApply "Hv"; eauto. }
+    iIntros (w); iDestruct 1 as (w') "[Hw #Hiw]".
+    iExists _; rewrite -interp_subst; eauto.
+  Qed.
+
+  Lemma bin_log_related_fold Γ e e' τ
+      (IHHtyped : Γ ⊨ e ≤log≤ e' : τ.[(TRec τ)/]) :
+    Γ ⊨ Fold e ≤log≤ Fold e' : TRec τ.
+  Proof.
+    iIntros (Δ vvs ρ ?) "#(Hh & Hs & HΓ)"; iIntros (K) "Hj /=".
+    iApply (wp_bind [FoldCtx]); iApply wp_wand_l; iSplitR;
+        [|iApply ('IHHtyped _ _ _ (K ++ [FoldCtx]));
+          rewrite ?fill_app; simpl; repeat iSplitR; trivial].
+    iIntros (v); iDestruct 1 as (w) "[Hv #Hiv]"; rewrite fill_app.
+    value_case. iExists (FoldV w); iFrame "Hv".
+    rewrite fixpoint_unfold /= -interp_subst.
+    iAlways; iExists (_, _); eauto.
+  Qed.
+
+  Lemma bin_log_related_unfold Γ e e' τ
+      (IHHtyped : Γ ⊨ e ≤log≤ e' : TRec τ) :
+    Γ ⊨ Unfold e ≤log≤ Unfold e' : τ.[(TRec τ)/].
+  Proof.
+    iIntros (Δ vvs ρ ?) "#(Hh & Hs & HΓ)"; iIntros (K) "Hj /=".
+    iApply (wp_bind [UnfoldCtx]); iApply wp_wand_l; iSplitR;
+        [|iApply ('IHHtyped _ _ _ (K ++ [UnfoldCtx]));
+          rewrite ?fill_app; simpl; repeat iSplitR; trivial].
+    iIntros (v). iDestruct 1 as (v') "[Hw #Hiw]"; rewrite fill_app.
+    rewrite /= fixpoint_unfold /=.
+    change (fixpoint _) with (interp (TRec τ) Δ).
+    iDestruct "Hiw" as ([w w']) "#[% Hiz]"; simplify_eq/=.
+    iMod (step_Fold _ _ K (of_val w') w' with "* [-]") as "Hz"; eauto.
+    iApply wp_fold; cbn; auto.
+    iNext; iModIntro; iExists _; iFrame "Hz". by rewrite -interp_subst.
+  Qed.
+
+  Lemma bin_log_related_alloc Γ e e' τ
+      (IHHtyped : Γ ⊨ e ≤log≤ e' : τ) :
+    Γ ⊨ Alloc e ≤log≤ Alloc e' : Tref τ.
+  Proof.
+    iIntros (Δ vvs ρ ?) "#(Hh & Hs & HΓ)"; iIntros (K) "Hj /=".
+    smart_wp_bind (AllocCtx) v v' "[Hv #Hiv]" ('IHHtyped _ _ _ (K ++ [AllocCtx])).
+    iMod (step_alloc _ _ K (of_val v') v' with "* [-]") as (l') "[Hj Hl]"; eauto.
+    iApply wp_fupd. iApply (wp_alloc with "[]"); auto.
+    iIntros "!>"; iIntros (l) "Hl'".
+    iMod (inv_alloc (logN .@ (l,l')) _ (∃ w : val * val,
+      l ↦ w.1 ∗ l' ↦ₛ w.2 ∗ interp τ Δ w)%I with "[Hl Hl']") as "HN"; eauto.
+    { iNext; iExists (v, v'); by iFrame. }
+    iModIntro; iExists (LocV l'). iFrame "Hj". iExists (l, l'); eauto.
+  Qed.
+
+  Lemma bin_log_related_load Γ e e' τ
+      (IHHtyped : Γ ⊨ e ≤log≤ e' : (Tref τ)) :
+    Γ ⊨ Load e ≤log≤ Load e' : τ.
+  Proof.
+    iIntros (Δ vvs ρ ?) "#(Hh & Hs & HΓ)"; iIntros (K) "Hj /=".
+    smart_wp_bind (LoadCtx) v v' "[Hv #Hiv]" ('IHHtyped _ _ _ (K ++ [LoadCtx])).
+    iDestruct "Hiv" as ([l l']) "[% Hinv]"; simplify_eq/=.
+    iInv (logN .@ (l,l')) as ([w w']) "[Hw1 [Hw2 #Hw]]" "Hclose"; simpl.
+    iMod "Hw2".
+    iMod (step_load _ _ K l' 1 w' with "[Hv Hw2]") as "[Hv Hw2]";
+      [solve_ndisj|by iFrame|].
+    iApply (wp_load _ _ 1 with "[Hw1]"); [|iFrame "Hh"|]; trivial; try solve_ndisj.
+    iNext. iIntros "Hw1". iMod ("Hclose" with "[Hw1 Hw2]").
+    { iNext. iExists (w,w'); by iFrame. }
+    iModIntro. iExists w'; by iFrame.
+  Qed.
+
+  Lemma bin_log_related_store Γ e1 e2 e1' e2' τ
+      (IHHtyped1 : Γ ⊨ e1 ≤log≤ e1' : (Tref τ))
+      (IHHtyped2 : Γ ⊨ e2 ≤log≤ e2' : τ) :
+    Γ ⊨ Store e1 e2 ≤log≤ Store e1' e2' : TUnit.
+  Proof.
+    iIntros (Δ vvs ρ ?) "#(Hh & Hs & HΓ)"; iIntros (K) "Hj /=".
+    smart_wp_bind (StoreLCtx _) v v' "[Hv #Hiv]"
+      ('IHHtyped1 _ _ _ (K ++ [StoreLCtx _])).
+    smart_wp_bind (StoreRCtx _) w w' "[Hw #Hiw]"
+      ('IHHtyped2 _ _ _ (K ++ [StoreRCtx _])).
+    iDestruct "Hiv" as ([l l']) "[% Hinv]"; simplify_eq/=.
+    iInv (logN .@ (l,l')) as ([v v']) "[>Hv1 [>Hv2 #Hv]]" "Hclose".
+    iMod (step_store _ _ K l' v' (of_val w') w' with "[Hw Hv2]")
+      as "[Hw Hv2]"; [eauto|solve_ndisj|by iFrame|].
+    iApply (wp_store with "[Hv1]"); auto using to_of_val. solve_ndisj.
+    iNext. iIntros "Hv1". iMod ("Hclose" with "[Hv1 Hv2]").
+    { iNext; iExists (w, w'); by iFrame. }
+    iExists UnitV; iFrame; auto.
+  Qed.
+
+  Theorem binary_fundamental Γ e τ :
+    Γ ⊢ₜ e : τ → Γ ⊨ e ≤log≤ e : τ.
+  Proof.
+    induction 1.
+    - by apply bin_log_related_var.
+    - by apply bin_log_related_unit.
+    - apply bin_log_related_pair; eauto.
+    - eapply bin_log_related_fst; eauto.
+    - eapply bin_log_related_snd; eauto.
+    - eapply bin_log_related_injl; eauto.
+    - eapply bin_log_related_injr; eauto.
+    - eapply bin_log_related_case; eauto;
+        match goal with H : _ |- _ => eapply (typed_n_closed _ _ _ H) end.
+    - eapply bin_log_related_lam; eauto;
+        match goal with H : _ |- _ => eapply (typed_n_closed _ _ _ H) end.
+    - eapply bin_log_related_app; eauto.
+    - eapply bin_log_related_tlam; eauto with typeclass_instances.
+    - eapply bin_log_related_tapp; eauto.
+    - eapply bin_log_related_fold; eauto.
+    - eapply bin_log_related_unfold; eauto.
+    - eapply bin_log_related_alloc; eauto.
+    - eapply bin_log_related_load; eauto.
+    - eapply bin_log_related_store; eauto.
+  Qed.
+End fundamental.
