F_mu_ref/rules_binary.v
@@ -1,0 +1,185 @@
+From iris.program_logic Require Import lifting.
+From iris.algebra Require Import frac dec_agree gmap list.
+From iris.base_logic Require Import big_op auth.
+From iris_logrel.F_mu_ref Require Export rules.
+From iris.proofmode Require Import tactics.
+Import uPred.
+
+Definition specN := nroot .@ "spec".
+
+(** The CMRA for the heap of the specification. *)
+Definition cfgUR := prodUR (optionUR (exclR exprC)) heapUR.
+
+(** The CMRA for the thread pool. *)
+Class cfgSG Σ :=
+  CFGSG { ctg_heapG :> heapG Σ; cfg_inG :> authG Σ cfgUR; cfg_name : gname }.
+
+Section definitionsS.
+  Context `{cfgSG Σ}.
+
+  Definition heapS_mapsto (l : loc) (q : Qp) (v: val) : iProp Σ :=
+    own cfg_name (◯ (∅, {[ l := (q, DecAgree v) ]})).
+
+  Definition tpool_mapsto (e: expr) : iProp Σ :=
+    own cfg_name (◯ (Excl' e, ∅)).
+
+  Definition spec_inv (ρ : cfg lang) : iProp Σ :=
+    (∃ e σ, own cfg_name (● (Excl' e , to_heap σ)) ∗ ■ rtc step ρ ([e],σ))%I.
+  Definition spec_ctx (ρ : cfg lang) : iProp Σ :=
+    inv specN (spec_inv ρ).
+
+  Global Instance heapS_mapsto_timeless l q v : TimelessP (heapS_mapsto l q v).
+  Proof. apply _. Qed.
+  Global Instance spec_ctx_persistent ρ : PersistentP (spec_ctx ρ).
+  Proof. apply _. Qed.
+End definitionsS.
+Typeclasses Opaque heapS_mapsto tpool_mapsto.
+
+Notation "l ↦ₛ{ q } v" := (heapS_mapsto l q v)
+  (at level 20, q at level 50, format "l  ↦ₛ{ q }  v") : uPred_scope.
+Notation "l ↦ₛ v" := (heapS_mapsto l 1 v) (at level 20) : uPred_scope.
+Notation "⤇ e" := (tpool_mapsto e) (at level 20) : uPred_scope.
+
+Section cfg.
+  Context `{cfgSG Σ}.
+  Implicit Types P Q : iProp Σ.
+  Implicit Types Φ : val → iProp Σ.
+  Implicit Types σ : state.
+  Implicit Types g : heapUR.
+  Implicit Types e : expr.
+  Implicit Types v : val.
+
+  (** Conversion to tpools and back *)
+  Lemma step_insert_no_fork K e σ e' σ' :
+    head_step e σ e' σ' [] → step ([fill K e], σ) ([fill K e'], σ').
+  Proof. intros Hst. eapply (step_atomic _ _ _ _ _ _ [] [] []); eauto.
+         by apply: Ectx_step'.
+  Qed.
+
+  Lemma step_pure E ρ K e e' :
+    (∀ σ, head_step e σ e' σ []) →
+    nclose specN ⊆ E →
+    spec_ctx ρ ∗ ⤇ fill K e ={E}=∗ ⤇ fill K e'.
+  Proof.
+    iIntros (??) "[#Hspec Hj]". rewrite /spec_ctx /tpool_mapsto.
+    iInv specN as ">Hinv" "Hclose". iDestruct "Hinv" as (e2 σ) "[Hown %]".
+    iDestruct (own_valid_2 _ with "[$Hown $Hj]")
+      as %[[?%Excl_included%leibniz_equiv _]%prod_included ?]%auth_valid_discrete_2.
+    subst.
+    iMod (own_update_2 with "[$Hown $Hj]") as "[Hown Hj]".
+    { by eapply auth_update, prod_local_update_1, option_local_update,
+       (exclusive_local_update _ (Excl (fill K e'))). }
+    iFrame "Hj". iApply "Hclose". iNext. iExists (fill K e'), σ.
+    iFrame. iPureIntro. eapply rtc_r, step_insert_no_fork; eauto.
+  Qed.
+
+  Lemma step_alloc E ρ K e v:
+    to_val e = Some v → nclose specN ⊆ E →
+    spec_ctx ρ ∗ ⤇ fill K (Alloc e) ={E}=∗ ∃ l, ⤇ fill K (Loc l) ∗ l ↦ₛ v.
+  Proof.
+    iIntros (??) "[#Hinv Hj]". rewrite /spec_ctx /tpool_mapsto.
+    iInv specN as ">Hinv'" "Hclose". iDestruct "Hinv'" as (e2 σ) "[Hown %]".
+    destruct (exist_fresh (dom (gset positive) σ)) as [l Hl%not_elem_of_dom].
+    iDestruct (own_valid_2 _ with "[$Hown $Hj]")
+      as %[[?%Excl_included%leibniz_equiv _]%prod_included ?]%auth_valid_discrete_2.
+    subst.
+    iMod (own_update_2 with "[$Hown $Hj]") as "[Hown Hj]".
+    { by eapply auth_update, prod_local_update_1, option_local_update,
+       (exclusive_local_update _ (Excl (fill K (Loc l)))). }
+    iMod (own_update with "Hown") as "[Hown Hl]".
+    { eapply auth_update_alloc, prod_local_update_2,
+        (alloc_singleton_local_update _ l (1%Qp,DecAgree v)); last done.
+      by apply lookup_to_heap_None. }
+    iExists l. rewrite /heapS_mapsto. iFrame "Hj Hl". iApply "Hclose". iNext.
+    iExists (fill K (Loc l)), (<[l:=v]>σ).
+    rewrite to_heap_insert; last eauto. iFrame. iPureIntro.
+    eapply rtc_r, step_insert_no_fork; eauto. econstructor; eauto.
+  Qed.
+
+  Lemma step_load E ρ K l q v:
+    nclose specN ⊆ E →
+    spec_ctx ρ ∗ ⤇ fill K (Load (Loc l)) ∗ l ↦ₛ{q} v
+    ={E}=∗ ⤇ fill K (of_val v) ∗ l ↦ₛ{q} v.
+  Proof.
+    iIntros (?) "(#Hinv & Hj & Hl)".
+    rewrite /spec_ctx /tpool_mapsto /heapS_mapsto.
+    iInv specN as ">Hinv'" "Hclose". iDestruct "Hinv'" as (e2 σ) "[Hown %]".
+    iDestruct (own_valid_2 _ with "[$Hown $Hj]")
+      as %[[?%Excl_included%leibniz_equiv _]%prod_included ?]%auth_valid_discrete_2.
+    subst.
+    iDestruct (own_valid_2 _ with "[$Hown $Hl]")
+      as %[[_ ?%heap_singleton_included]%prod_included _]%auth_valid_discrete_2.
+    iMod (own_update_2 with "[$Hown $Hj]") as "[Hown Hj]".
+    { by eapply auth_update, prod_local_update_1, option_local_update,
+        (exclusive_local_update _ (Excl (fill K (of_val v)))). }
+    iFrame "Hj Hl". iApply "Hclose". iNext.
+    iExists (fill K (of_val v)), σ.
+    iFrame. iPureIntro.
+    eapply rtc_r, step_insert_no_fork; eauto. econstructor; eauto.
+  Qed.
+
+  Lemma step_store E ρ K l v' e v:
+    to_val e = Some v → nclose specN ⊆ E →
+    spec_ctx ρ ∗ ⤇ fill K (Store (Loc l) e) ∗ l ↦ₛ v'
+    ={E}=∗ ⤇ fill K Unit ∗ l ↦ₛ v.
+  Proof.
+    iIntros (??) "(#Hinv & Hj & Hl)".
+    rewrite /spec_ctx /tpool_mapsto /heapS_mapsto.
+    iInv specN as ">Hinv'" "Hclose". iDestruct "Hinv'" as (e2 σ) "[Hown %]".
+    iDestruct (own_valid_2 _ with "[$Hown $Hj]")
+      as %[[?%Excl_included%leibniz_equiv _]%prod_included ?]%auth_valid_discrete_2.
+    subst.
+    iDestruct (own_valid_2 _ with "[$Hown $Hl]")
+      as %[[_ Hl%heap_singleton_included]%prod_included _]%auth_valid_discrete_2.
+    iMod (own_update_2 with "[$Hown $Hj]") as "[Hown Hj]".
+    { by eapply auth_update, prod_local_update_1, option_local_update,
+        (exclusive_local_update _ (Excl (fill K Unit))). }
+    iMod (own_update_2 with "[$Hown $Hl]") as "[Hown Hl]".
+    { eapply auth_update, prod_local_update_2, singleton_local_update,
+        (exclusive_local_update _ (1%Qp, DecAgree v)); last done.
+      by rewrite /to_heap lookup_fmap Hl. }
+    iFrame "Hj Hl". iApply "Hclose". iNext.
+    iExists (fill K Unit), (<[l:=v]>σ).
+    rewrite to_heap_insert; last eauto. iFrame. iPureIntro.
+    eapply rtc_r, step_insert_no_fork; eauto. econstructor; eauto.
+  Qed.
+
+  Lemma step_lam E ρ K e1 e2 v :
+    to_val e2 = Some v → nclose specN ⊆ E →
+    spec_ctx ρ ∗ ⤇ fill K (App (Lam e1) e2)
+    ={E}=∗ ⤇ fill K (e1.[e2/]).
+  Proof. intros ?; apply step_pure => σ; econstructor; eauto. Qed.
+
+  Lemma step_tlam E ρ K e :
+    nclose specN ⊆ E →
+    spec_ctx ρ ∗ ⤇ fill K (TApp (TLam e)) ={E}=∗ ⤇ fill K e.
+  Proof. apply step_pure => σ; econstructor; eauto. Qed.
+
+  Lemma step_Fold E ρ K e v :
+    to_val e = Some v → nclose specN ⊆ E →
+    spec_ctx ρ ∗ ⤇ fill K (Unfold (Fold e)) ={E}=∗ ⤇ fill K e.
+  Proof. intros H1; apply step_pure => σ; econstructor; eauto. Qed.
+
+  Lemma step_fst E ρ K e1 v1 e2 v2 :
+    to_val e1 = Some v1 → to_val e2 = Some v2 → nclose specN ⊆ E →
+    spec_ctx ρ ∗ ⤇ fill K (Fst (Pair e1 e2)) ={E}=∗ ⤇ fill K e1.
+  Proof. intros H1 H2; apply step_pure => σ; econstructor; eauto. Qed.
+
+  Lemma step_snd E ρ K e1 v1 e2 v2 :
+    to_val e1 = Some v1 → to_val e2 = Some v2 → nclose specN ⊆ E →
+    spec_ctx ρ ∗ ⤇ fill K (Snd (Pair e1 e2)) ={E}=∗ ⤇ fill K e2.
+  Proof. intros H1 H2; apply step_pure => σ; econstructor; eauto. Qed.
+
+  Lemma step_case_inl E ρ K e0 v0 e1 e2 :
+    to_val e0 = Some v0 → nclose specN ⊆ E →
+    spec_ctx ρ ∗ ⤇ fill K (Case (InjL e0) e1 e2)
+      ={E}=∗ ⤇ fill K (e1.[e0/]).
+  Proof. intros H1; apply step_pure => σ; econstructor; eauto. Qed.
+
+  Lemma step_case_inr E ρ K e0 v0 e1 e2 :
+    to_val e0 = Some v0 → nclose specN ⊆ E →
+    spec_ctx ρ ∗ ⤇ fill K (Case (InjR e0) e1 e2)
+      ={E}=∗ ⤇ fill K (e2.[e0/]).
+  Proof. intros H1; apply step_pure => σ; econstructor; eauto. Qed.
+
+End cfg.
