README.md
@@ -5,4 +5,4 @@ This version is known to compile with:
  - Coq 8.5pl2
  - Ssreflect 1.6
  - Autosubst 1.5
- - Iris version https://gitlab.mpi-sws.org/FP/iris-coq/commit/37cf94e2
+ - Iris version https://gitlab.mpi-sws.org/FP/iris-coq/commit/2a7755f
